started server-side negotiation; fixed a version-formatting bug in HandshakeMessages

src/tls/Negotiation.fst
@@ -25,7 +25,7 @@ val discard: bool -> ST unit
   (requires (fun _ -> True))
   (ensures (fun h0 _ h1 -> h0 == h1))
 let discard _ = ()
-let print s = discard (IO.debug_print_string ("HS | "^s^"\n"))
+let print s = discard (IO.debug_print_string ("NGO| "^s^"\n"))
 unfold val trace: s:string -> ST unit
   (requires (fun _ -> True))
   (ensures (fun h0 _ h1 -> h0 == h1))
@@ -91,7 +91,7 @@ noeq type mode =
     // more from SH (both TLS 1.2 and TLS 1.3)
     n_protocol_version: protocolVersion ->
     n_server_random: TLSInfo.random ->
-    n_sessionID: option sessionID -> // optional 1.2 id for *future* resumptions (not always what SH carries)
+    n_sessionID: option sessionID {n_sessionID = None <==> n_protocol_version = TLS_1p3} -> 
     n_cipher_suite: cipherSuite ->
 
     // concatenating SH and EE extensions for 1.3, in wire order.
@@ -109,6 +109,16 @@ noeq type mode =
     // { both shares are in the same negotiated group }
     mode
 
+let is_resumption12 m = 
+  m.n_protocol_version <> TLS_1p3  &&
+  m.n_sessionID = Some (m.n_offer.ch_sessionID)
+
+let is_cacheable12 m = 
+  m.n_protocol_version <> TLS_1p3  &&
+  ( let Some sid = m.n_sessionID in
+    sid <> m.n_offer.ch_sessionID &&
+    sid <> empty_bytes)
+
 // 17-04-25 we need pure functions of the mode for these old fields 
 //    n_resume: option bool -> // is this a 1.2 resumption with the offered sid?
 //    n_psk: option PSK.pskid -> // none with 1.2 (we are not doing PSK 1.2)
@@ -121,7 +131,7 @@ noeq type mode =
 // and for each of the fields of
 //    n_extensions: negotiatedExtensions ->
 
-let client_sigalg_extension (m:mode) = 
+let client_sigalg_extension (m:mode) : option (list sigHashAlg) = 
   match m.n_offer.ch_extensions with
   | None -> None 
   | Some es -> 
@@ -129,21 +139,30 @@ let client_sigalg_extension (m:mode) =
     | None -> None 
     | Some (E_signature_algorithms sas) -> Some sas 
 
+// Signature agility, depending on the CS and an optional client extension
 let sig_algs (m: mode) (ha0: TLSConstants.hashAlg) = 
-  // Signature agility (following the broken rules of 7.4.1.4.1. in RFC5246)
-  // If no signature nego took place we use the SA and KDF hash from the CS
-  let CipherSuite _ (Some sa) _ = m.n_cipher_suite in
   let sa, ha = 
-    match client_sigalg_extension m with
-    | None -> sa, ha0  
-    | Some algs -> 
-        match List.Tot.find (fun (s,_) -> s = sa) algs with
-        | Some sa_ha -> sa_ha
-        | None -> sa, ha0 in 
+    if m.n_protocol_version = TLS_1p3 
+    then 
+      // the extension is required for signing
+      // https://tlswg.github.io/tls13-spec/#rfc.section.4.2.3 
+      // TO BE COMPLETED
+      let Some ((sa,ha)::_) = client_sigalg_extension m in
+      (sa, ha)
+    else 
+      // If no signature nego took place we use the SA and KDF hash from the CS
+      // otherwise we still follow the SA and only use the extension to pick the hash
+      // (is it too conservative?)
+      // https://tools.ietf.org/html/rfc5246#section-7.4.1.4.1 
+      let CipherSuite _ (Some sa) _ = m.n_cipher_suite in
+      ( match client_sigalg_extension m with
+        | None -> sa, ha0  
+        | Some algs -> 
+          match List.Tot.find (fun (s,_) -> s = sa) algs with
+          | Some sa_ha -> sa_ha
+          | None -> (sa, ha0)) in
   let a = Signature.(Use (fun _ -> true) sa [ha] false false) in
   (a, sa, ha)
-//17-04-25 we seem to unduly respect the signature algorithm for the CS
-//17-04-25 on the server side, this should depend on the certs we have!
 
 noeq type negotiationState (r:role) (cfg:config) (resume:resumeInfo r) =
   // Have C_Offer_13 and C_Offer? Shares aren't available in C_Offer yet
@@ -343,15 +362,46 @@ let client_ClientHello #region ns oks =
       offer
 
 (**
-  Checks that the protocol version in the CHELO message is
+  Checks that the protocol version in ClientHello is
   within the range of versions supported by the server configuration
   and outputs the negotiated version if true
 *)
-val negotiateVersion: cfg:config -> c:protocolVersion -> Tot (result protocolVersion)
-let negotiateVersion cfg c =
-  if geqPV c cfg.minVer && geqPV cfg.maxVer c then Correct c
-  else if geqPV c cfg.maxVer then Correct cfg.maxVer
-  else Error(AD_internal_error, perror __SOURCE_FILE__ __LINE__ "Protocol version negotiation failed")
+  
+// usable on both sides; following https://tlswg.github.io/tls13-spec/#rfc.section.4.2.1 
+let offered_versions min_pv (o: offer): result (l: list protocolVersion {l <> []}) =
+  let extent = 
+    match o.ch_extensions with
+    | None -> None 
+    | Some es -> 
+      match List.Tot.find Extensions.E_supported_versions? es with
+      | None -> None 
+      | Some (Extensions.E_supported_versions vs) -> Some vs in
+  match extent with 
+  | Some []  -> Error(AD_internal_error, "protocol version negotiation: empty proposal")
+  | Some vs -> Correct vs  // might check no proposal is below min_pv
+  | None -> // use legacy offer
+      match o.ch_protocol_version, min_pv with 
+      | TLS_1p0, TLS_1p0 -> Correct [TLS_1p0] 
+      | TLS_1p1, TLS_1p0 -> Correct [TLS_1p2; TLS_1p1] 
+      | TLS_1p1, TLS_1p1 -> Correct [TLS_1p1] 
+      | TLS_1p2, TLS_1p0 -> Correct [TLS_1p2; TLS_1p1; TLS_1p0] 
+      | TLS_1p2, TLS_1p1 -> Correct [TLS_1p2; TLS_1p1] 
+      | TLS_1p2, TLS_1p2 -> Correct [TLS_1p2] 
+      | _, _ -> Error(AD_internal_error, "protocol version negotation: bad legacy proposal")
+
+let is_client13 (o:offer) = 
+  match offered_versions TLS_1p3 o with 
+  | Correct vs -> List.Tot.existsb (fun v -> v = TLS_1p3) vs 
+  | Error _ -> false 
+
+let negotiate_version cfg offer = 
+  //17-04-26 TODO pass outer packet PV instead of TLS_1p2
+  match offered_versions TLS_1p2 offer with 
+  | Error z -> Error z 
+  | Correct vs -> 
+    match List.Tot.find (fun v -> geqPV cfg.maxVer v && geqPV cfg.minVer v) vs with 
+    | Some v -> Correct v
+    | None -> Error(AD_internal_error, "protocol version negotiation: mismatch")
 
 (**
   For use in negotiating the ciphersuite, takes two lists and
@@ -374,7 +424,7 @@ let negotiateCipherSuite cfg pv ccs =
   | None -> Error(AD_internal_error, perror __SOURCE_FILE__ __LINE__ "Cipher suite negotiation failed")
 
 assume
-val negotiateGroupKeyShare: config -> protocolVersion -> TLSConstants.kexAlg -> option (list extension) -> Tot (result (option namedGroup * option bytes))
+val negotiateGroupKeyShare: config -> protocolVersion -> TLSConstants.kexAlg -> list extension -> Tot (result (option namedGroup * option bytes))
 (*
 let rec negotiateGroupKeyShare cfg pv kex exts =
   match exts with
@@ -426,13 +476,13 @@ let isSentinelRandomValue c_pv s_pv s_random =
   - is not an unnecessary downgrade AND
   - is not a newer version than offered by the client
 *)
-val acceptableVersion: config -> protocolVersion -> protocolVersion -> TLSInfo.random -> Tot bool
-let acceptableVersion cfg cpv spv sr =
-  match negotiateVersion cfg cpv with
-  | Correct c_pv ->
-    geqPV c_pv spv && geqPV spv cfg.minVer &&
-    not (isSentinelRandomValue c_pv spv sr)
-  | Error _ -> false
+val acceptableVersion: config -> protocolVersion -> TLSInfo.random -> Tot bool
+let acceptableVersion cfg pv sr =
+  // we statically know that the offered versions are compatible with our config
+  // (we may prove e.g. acceptableVersion pv ==> pv in offered_versions
+  geqPV pv cfg.minVer && 
+  geqPV cfg.maxVer pv &&
+  not (isSentinelRandomValue cfg.maxVer pv sr)
 
 (** Confirms that the ciphersuite negotiated by the server was:
   - consistent with the client config;
@@ -481,7 +531,7 @@ let client_ServerHello #region ns sh =
     let sig  = CoreCrypto.RSASIG in
     let resume = false in
     trace ("processing server extensions "^string_of_option_extensions sext);
-    if not (acceptableVersion ns.cfg ns.cfg.maxVer spv sr) then
+    if not (acceptableVersion ns.cfg spv sr) then
       Error(AD_illegal_parameter, perror __SOURCE_FILE__ __LINE__ "Protocol version negotiation")
     else if not (acceptableCipherSuite ns.cfg spv cs) then
       Error(AD_illegal_parameter, perror __SOURCE_FILE__ __LINE__ "Ciphersuite negotiation")
@@ -583,12 +633,6 @@ assume val clientComplete_13: #region:rgn -> #role:TLSConstants.role -> t region
 
 (* SERVER *)
 
-//HS: similar to computeServerMode
-assume val server_ClientHello: #region:rgn -> #role:TLSConstants.role -> t region role ->
-  HandshakeMessages.ch ->
-  sessionID -> 
-  St (result mode)
-
 //17-03-30 still missing a few for servers.
 
 // TODO ADL: incorrect as written; CS nego depends on ext nego
@@ -604,14 +648,22 @@ assume val server_ClientHello: #region:rgn -> #role:TLSConstants.role -> t regio
 // in between negotiating the named Group and preparing the
 // negotiated Extensions
 (* TODO: why irreducible? *)
-irreducible val computeServerMode: cfg:config -> cpv:protocolVersion -> ccs:valid_cipher_suites -> cexts:option (list extension) -> comps: (list compression) -> ri:option (cVerifyData*sVerifyData) -> Tot (result mode)
-let computeServerMode cfg cpv ccs cexts comps ri =
-  (match (negotiateVersion cfg cpv) with
-    | Error(z) -> Error(z)
-    | Correct(npv) ->
+irreducible val computeServerMode: 
+  cfg: config -> co: offer -> 
+  serverRandom: TLSInfo.random -> serverID: option sessionID -> 
+  Tot (result mode)
+let computeServerMode cfg co serverRandom serverID = 
+  // for now, we set the version before negotiating the rest; this may lead to mismatches e.g. on tickets or certificates
+  match negotiate_version cfg co with
+  | Error z -> Error z
+  | Correct pv ->
+
+  // with TLS 1.2, we pick the first ciphersuite compatible with our credentials
+  // we could be a bit stricter and record wether the client is TLS
   let nosa = fun (CipherSuite _ sa _) -> None? sa in
-  let sigfilter = match Cert.lookup_chain cfg.cert_chain_file with
-    | Correct(c) when (Some? (Cert.endpoint_keytype c)) ->
+  let sigfilter = 
+    match Cert.lookup_chain cfg.cert_chain_file with
+    | Correct c when (Some? (Cert.endpoint_keytype c)) ->
       let kt = Cert.endpoint_keytype c in
       (fun (CipherSuite _ sa _) ->
         match sa,kt with
@@ -627,48 +679,79 @@ let computeServerMode cfg cpv ccs cexts comps ri =
           IO.debug_print_string "WARNING cannot load server cert; restricting to anonymous CS...\n"
         else false in
        nosa in
-  let ccs = List.Tot.filter sigfilter ccs in
-  match negotiateCipherSuite cfg npv ccs with
-    | Error(z) -> Error(z)
-    | Correct(kex,sa,ae,cs) ->
-  let nego = ne_default in
-  let next = (match cexts with
-   | Some cexts -> Correct(List.Tot.fold_left (clientToNegotiatedExtension cfg cs ri false) nego cexts)
-//   | None -> ne_default)
-   | None -> (match npv with
+  let ccs = List.Tot.filter sigfilter co.ch_cipher_suites in
+  match negotiateCipherSuite cfg pv ccs with
+  | Error z -> Error z
+  | Correct (kex,sa,ae,cs) ->
+
+  // compute server extensions
+  match co.ch_extensions with
+  | None -> Error(AD_illegal_parameter, "Missing mandatory ClientHello extensions")
+  (* omitted details: 
               | SSL_3p0 ->
                 let cre =
                   if contains_TLS_EMPTY_RENEGOTIATION_INFO_SCSV (list_valid_cs_is_list_cs ccs) then
                      {ne_default with ne_secure_renegotiation = RI_Valid}
                   else ne_default
                 in Correct (cre)
-             | _ -> Error(AD_internal_error, perror __SOURCE_FILE__ __LINE__ "Missing extensions in TLS client hello")))
-  in
-  let ng = negotiateGroupKeyShare cfg npv kex cexts in
-  match next, ng with
-    | Error(z), _ | _, Error(z) -> Error(z)
-    | Correct(next), Correct(gn, gxo) ->
-      let comp = match comps with
-                 | [] -> None
-                 | _ -> Some NullCompression in
-      let mode = admit () in
-      (*{
-        sm_protocol_version = npv;
-        sm_kexAlg = kex;
-        sm_aeAlg = ae;
-        sm_sigAlg = sa;
-        sm_cipher_suite = cs;
-        sm_dh_group = gn;
-        sm_dh_share = gxo;
-        sm_comp = comp;
-        sm_ext = next;
-      } in *)
-      Correct (mode))
+             | _ -> Error... )) *)
+  | Some cexts -> 
+(*
+  match Extensions.negotiateServerExtensions pv cexts with 
+  | Error z -> Error z 
+  | Correct serverExtensions -> 
+//    List.Tot.fold_left (Extensions.clientToNegotiatedExtension cfg cs None false) nego cexts 
+*)
+  let serverExtensions = Some [] in 
+
+  match negotiateGroupKeyShare cfg pv kex cexts with 
+  | Error z -> Error z 
+  | Correct (ng,gxo) ->
+
+  // compression is null and non-negotiable; we just report client errors
+  let correct_compression_offer = 
+    if is_client13 co 
+    then co.ch_compressions = [NullCompression] 
+    else List.Tot.existsb (fun c -> c = NullCompression) co.ch_compressions in
+  if not correct_compression_offer 
+  then Error(AD_illegal_parameter, "Compression is deprecated") else 
+
+  Correct (Mode
+    co
+    None //TODO: support HRR 
+    pv
+    serverRandom
+    serverID
+    cs
+    serverExtensions
+    None // no server key share yet
+    None // no client request yet
+    None // no server cert yet
+    None // no client key share yet
+  )
+  
+//HS: similar to computeServerMode
+val server_ClientHello: #region:rgn -> t region Server ->
+  HandshakeMessages.ch ->
+  option sessionID -> 
+  St (result mode)
+let server_ClientHello #region ns offer sid =
+  match MR.m_read ns.state with 
+  | S_Init _ -> 
+      match computeServerMode ns.cfg offer ns.nonce sid with
+      | Error z -> 
+          trace ("negotiation failed: "^string_of_error z); 
+          Error z
+      | Correct m -> 
+          trace ("including server extensions "^string_of_option_extensions m.n_server_extensions);
+          MR.m_write ns.state (C_Offer offer);
+          Correct m
+
 
 
 irreducible val computeClientMode: cfg:config -> cext:option (list extension) -> cpv:protocolVersion -> spv:protocolVersion -> sr:TLSInfo.random -> cs:valid_cipher_suite -> sext:option (list extension) -> comp:option compression -> option ri -> Tot (result mode)
 let computeClientMode cfg cext cpv spv sr cs sext comp ri =
-  if not (acceptableVersion cfg cpv spv sr) then
+  if not (acceptableVersion cfg spv sr) then
     Error(AD_illegal_parameter, perror __SOURCE_FILE__ __LINE__ "Protocol version negotiation")
   else if not (acceptableCipherSuite cfg spv cs) then
     Error(AD_illegal_parameter, perror __SOURCE_FILE__ __LINE__ "Ciphersuite negotiation")
